fix formatting, update to work with new List.scanlM

Batteries/Data/Iterators/Scan.lean
@@ -14,24 +14,26 @@ namespace Std.Iterators
 /--
   Internal state for the ScanM combinator
 -/
-structure ScanM (α : Type w) (m : Type w → Type w') (n : Type w → Type w'') (β : Type w) (γ : Type w)
-    (f : γ → β → n γ) where
+structure ScanM (α : Type w) (m : Type w → Type w') (n : Type w → Type w'')
+    (β : Type w) (γ : Type w) (f : γ → β → n γ) where
   /-- Inner iterator -/
   inner : α
   /-- Current accumulated value -/
   acc : γ
-  /-- Whether we have emitted the initial value (and therefore should begin yielding from the iterator) -/
+  /-- Whether we have emitted the initial value
+    (and therefore should begin yielding from the iterator) -/
   emittedInit : Bool
 
 namespace ScanM
 
-variable {α β γ : Type w} {m : Type w → Type w'} {n : Type w → Type w''} {f : γ → β → n γ} [Iterator α m β]
+variable {α β γ : Type w} {m : Type w → Type w'} {n : Type w → Type w''}
+  {f : γ → β → n γ} [Iterator α m β]
 /--
-`it.IsPlausibleStep` is the proposition that `step` is a possible next step from the `scanM` iterator `it`.
-This is mostly an internal implementation detail used to prove termination.
+`it.IsPlausibleStep` is the proposition that `step` is a possible next step from the `scanM`
+iterator `it`. This is mostly an internal implementation detail used to prove termination.
 -/
-inductive IsPlausibleStep
-    (it : @IterM (ScanM α m n β γ f) n γ) : IterStep (@IterM (ScanM α m n β γ f) n γ) γ → Prop where
+inductive IsPlausibleStep (it : @IterM (ScanM α m n β γ f) n γ) :
+    IterStep (@IterM (ScanM α m n β γ f) n γ) γ → Prop where
 
   /-- If we haven't emitted anything yet (emittedInit is false),
       we set it to true and do not update the internal iterator state
@@ -63,7 +65,6 @@ inductive IsPlausibleStep
       it.internalState.emittedInit = true →
       Iterator.IsPlausibleStep (⟨it.internalState.inner⟩ : IterM m β) .done →
       IsPlausibleStep it .done
-
 
 instance instIterator [Monad n] [MonadLiftT m n] :
     Iterator (ScanM α m n β γ f) n γ where
@@ -103,7 +104,8 @@ instance {o : Type w → Type x} [Monad n] [MonadLiftT m n] [Monad o] [MonadLift
 private def finRel (scanIt' scanIt : @IterM (ScanM α m n β γ f) n γ) : Prop :=
   match scanIt.internalState.emittedInit, scanIt'.internalState.emittedInit with
   | false, true => True
-  | true, true => (⟨scanIt'.internalState.inner⟩ : IterM m β).IsPlausibleSuccessorOf ⟨scanIt.internalState.inner⟩
+  | true, true => (⟨scanIt'.internalState.inner⟩ : IterM m β).IsPlausibleSuccessorOf
+      ⟨scanIt.internalState.inner⟩
   | _, _ => False
 
 private theorem acc_finRel_emittedTrue [Finite α m (β := β)]
@@ -130,12 +132,11 @@ private theorem acc_finRel_emittedFalse [Finite α m (β := β)]
     -- this leads to a contradiction
     . simp_all [finRel]
 
-
-private theorem acc_finRel [Finite α m (β := β)] (scanIt : @IterM (ScanM α m n β γ f) n γ) : Acc finRel scanIt :=
+private theorem acc_finRel [Finite α m (β := β)] (scanIt : @IterM (ScanM α m n β γ f) n γ) :
+    Acc finRel scanIt :=
   if h : scanIt.internalState.emittedInit
     then acc_finRel_emittedTrue _ ‹_›
     else acc_finRel_emittedFalse _ (by simp only [h])
-
 
 private instance instFinRel [Monad m] [Monad n] [MonadLiftT m n] [Finite α m (β := β)] :
     FinitenessRelation (ScanM α m n β γ f) n where
@@ -150,20 +151,19 @@ private instance instFinRel [Monad m] [Monad n] [MonadLiftT m n] [Finite α m (�
     . exact IterM.isPlausibleSuccessorOf_of_yield ‹_›
     . exact IterM.isPlausibleSuccessorOf_of_skip  ‹_›
 
-instance [Finite α m (β := β)] [Monad m] [Monad n] [MonadLiftT m n] : Finite (ScanM α m n β γ f) n :=
+instance [Finite α m (β := β)] [Monad m] [Monad n] [MonadLiftT m n] :
+    Finite (ScanM α m n β γ f) n :=
   .of_finitenessRelation instFinRel
-
 
 /-- Productiveness relation for ScanM -/
 private def prodRel (scanIt' scanIt : @IterM (ScanM α m n β γ f) n γ) : Prop :=
   (⟨scanIt'.internalState.inner⟩ : IterM m β).IsPlausibleSkipSuccessorOf ⟨scanIt.internalState.inner⟩
 
 private theorem acc_prodRel [Productive α m (β := β)]
-    (scanIt : @IterM (ScanM α m n β γ f) n γ)
-  : Acc prodRel scanIt
-  := by
-    generalize hgen : (⟨scanIt.internalState.inner⟩ : IterM m β) = innerIt
-    induction Productive.wf.apply innerIt generalizing scanIt with grind only [prodRel, Acc]
+    (scanIt : @IterM (ScanM α m n β γ f) n γ) :
+    Acc prodRel scanIt := by
+  generalize hgen : (⟨scanIt.internalState.inner⟩ : IterM m β) = innerIt
+  induction Productive.wf.apply innerIt generalizing scanIt with grind only [prodRel, Acc]
 
 private instance instProdRel [Monad m] [Monad n] [MonadLiftT m n] [Productive α m (β := β)] :
     ProductivenessRelation (ScanM α m n β γ f) n where
@@ -173,11 +173,11 @@ private instance instProdRel [Monad m] [Monad n] [MonadLiftT m n] [Productive α
     intro _ _ hsucc
     cases hsucc <;> simp_all [prodRel, IterM.IsPlausibleSkipSuccessorOf]
 
-instance [Productive α m (β := β)] [Monad m] [Monad n] [MonadLiftT m n] : Productive (ScanM α m n β γ f) n :=
+instance [Productive α m (β := β)] [Monad m] [Monad n] [MonadLiftT m n] :
+    Productive (ScanM α m n β γ f) n :=
   .of_productivenessRelation instProdRel
 
 end ScanM
-
 
 section Combinators
 variable {α β γ : Type w}
